spec/abstract/SchedContext_A.thy
@@ -294,11 +294,17 @@ where
 
 text \<open>consumed related functions\<close>
 
-definition sched_context_update_consumed :: "obj_ref \<Rightarrow> (time,'z::state_ext) s_monad" where
+definition sched_context_update_consumed :: "obj_ref \<Rightarrow> (time, 'z::state_ext) s_monad" where
   "sched_context_update_consumed sc_ptr \<equiv> do
      sc \<leftarrow> get_sched_context sc_ptr;
-     set_sc_obj_ref sc_consumed_update sc_ptr 0;
-     return (ticks_to_us (sc_consumed sc))
+     consumed \<leftarrow> return (sc_consumed sc);
+     if max_ticks_to_us \<le> consumed
+     then do set_sc_obj_ref sc_consumed_update sc_ptr (consumed - max_ticks_to_us);
+             return (ticks_to_us (max_ticks_to_us))
+          od
+     else do set_sc_obj_ref sc_consumed_update sc_ptr 0;
+             return (ticks_to_us (sc_consumed sc))
+          od
    od"
 
 definition set_consumed :: "obj_ref \<Rightarrow> obj_ref \<Rightarrow> (unit, 'z::state_ext) s_monad" where
